$
  abs(W( a + (b - a) / (2 n)))
  & = ((b - a)^(n + 1) (2n)!) / (2^(2n + 1) n^(n + 1) n!) \
  & >= ((b - a)^(n + 1) sqrt(4 pi n) ((2n) / e)^(2n)) / (2^(2n + 1) n^(n + 1) sqrt(2pi n) (n / e)^n) \
  & = ((b - a)^(n + 1) sqrt(2) dot 2^(2n) ((n) / e)^(2n)) / (2^(2n + 1) n^(n + 1) (n / e)^n) \
  & = ((b - a)^(n + 1) sqrt(2) dot n^n) / (2 dot n^(n + 1) e^n) \
  & = ((b - a)^(n + 1) sqrt(2)) / (2n e^n) \
  & = (b - a) sqrt(2) / 2 1/n ((b - a)/e)^n \
  & = c/n ((b - a)/e)^n "where" c = (b - a) sqrt(2) / 2 \
$
